examples.v
@@ -1,0 +1,582 @@
+Require Import main.
+Require Import List.
+Import ListNotations.
+Import rhs.exports.
+Import nfa_epsilon_transitions.exports.
+Require Import Classes.EquivDec.
+Require Import Coq.Program.Program.
+Require Import Bool.
+Require Import ListSet.
+
+Module non_terminal.
+    Inductive t:Type :=
+      A | B.
+
+Obligation Tactic := unfold complement, equiv ; program_simpl.
+    Program Instance eqdec : EqDec t eq :=
+      { equiv_dec x y :=
+          match x, y with
+          | A, A => in_left
+          | B, B => in_left
+          | A, B | B, A => in_right
+          end
+      }.
+  End non_terminal.
+
+  Module terminal.
+    Inductive t : Type :=
+      a | b.
+
+    Program Instance eqdec : EqDec t eq :=
+      { equiv_dec x y :=
+          match x, y with
+          | a, a => in_left
+          | b, b => in_left
+          | a, b | b, a => in_right
+          end
+      }.
+  End terminal.
+
+  Definition a_b_rules: set (non_terminal.t * rhs.t terminal.t non_terminal.t):=
+    [(non_terminal.A, Continue terminal.a non_terminal.A);
+     (non_terminal.A, Continue terminal.b non_terminal.B);
+     (non_terminal.A, Empty);
+     (non_terminal.B, Continue terminal.b non_terminal.B);
+     (non_terminal.B, Empty)].
+
+  Definition a_b_grammar : reg_grammar.g terminal.t non_terminal.t :=
+    {| reg_grammar.start_symbol := non_terminal.A;
+       reg_grammar.rules := a_b_rules;
+       reg_grammar.terminal_symbols := [terminal.a;terminal.b];
+       reg_grammar.nonterminal_symbols := [non_terminal.A; non_terminal.B] |}.
+
+  (* A few examples. *)
+  Eval compute in reg_grammar.parse a_b_grammar [].
+  Eval compute in reg_grammar.parse a_b_grammar [terminal.a].
+  Eval compute in reg_grammar.parse a_b_grammar [terminal.a; terminal.a].
+  Eval compute in reg_grammar.parse a_b_grammar [terminal.b; terminal.b].
+  Eval compute in reg_grammar.parse a_b_grammar [terminal.a; terminal.b].
+  Eval compute in reg_grammar.parse a_b_grammar [terminal.b; terminal.a].
+
+  (*An NFA built from the grammar given above *)
+
+  Definition nfa_from_a_b_grammar := grammar_to_nfa.build_nfa_from_grammar a_b_grammar.
+  Eval compute in nfa.path nfa_from_a_b_grammar [].
+  Eval compute in nfa.run nfa_from_a_b_grammar [terminal.a; terminal.a;terminal.b; terminal.a].
+  Eval compute in nfa.run nfa_from_a_b_grammar [terminal.a; terminal.a].
+  Eval compute in nfa.run nfa_from_a_b_grammar [terminal.a; terminal.b].
+  Eval compute in nfa.run nfa_from_a_b_grammar [terminal.b; terminal.a].
+  Eval compute in nfa.states nfa_from_a_b_grammar.
+
+  (* A hand rolled DFA for the same language. *)
+  Definition a_b_next (s : option non_terminal.t) (t : terminal.t) : option non_terminal.t :=
+    match s with
+    | None => None
+    | Some non_terminal.A =>
+      match t with
+      | terminal.a => Some non_terminal.A
+      | terminal.b => Some non_terminal.B
+      end
+    | Some non_terminal.B =>
+      match t with
+      | terminal.a => None
+      | terminal.b => Some non_terminal.B
+      end
+    end.
+
+  Definition a_b_is_final (s : option non_terminal.t) : bool :=
+    match s with
+    | None => false
+    | Some _ => true
+    end.
+
+  Definition a_b_states := [Some non_terminal.A; Some non_terminal.B].
+
+  Definition a_b_dfa : dfa.t _ _  :=
+    {| dfa.initial_state := Some non_terminal.A;
+       dfa.is_final := a_b_is_final;
+       dfa.next := a_b_next;
+       dfa.states := a_b_states;
+       dfa.alphabet := [terminal.a;terminal.b] |}.
+
+
+  Extraction a_b_dfa.
+
+  (* Examples running the DFA. *)
+  Eval compute in dfa.run a_b_dfa [].
+  Eval compute in dfa.run a_b_dfa [terminal.a].
+  Eval compute in dfa.run a_b_dfa [terminal.b].
+  Eval compute in dfa.run a_b_dfa [terminal.a; terminal.a].
+  Eval compute in dfa.run a_b_dfa [terminal.b; terminal.b].
+  Eval compute in dfa.run a_b_dfa [terminal.a; terminal.b].
+  Eval compute in dfa.run a_b_dfa [terminal.b; terminal.b;terminal.a].
+  Eval compute in dfa.path a_b_dfa [terminal.b;terminal.b;terminal.a;terminal.a].
+  Definition xy := dfa.dfa_to_regular_grammar a_b_dfa.
+  Eval compute in reg_grammar.rules (xy).
+  Eval compute in reg_grammar.nonterminal_symbols xy.
+
+  (* Automatically construct a DFA using the powerset construction. *)
+  Check a_b_grammar.
+  Definition a_b_dfa' := powerset_construction.build_dfa a_b_grammar.
+  Eval compute in dfa.states a_b_dfa'.
+  Check a_b_dfa'.
+  Eval compute in reg_grammar.nonterminal_symbols a_b_grammar.
+  Eval compute in dfa.dfa_transitions_to_grammar_rules a_b_dfa'
+  (dfa.states a_b_dfa') (dfa.alphabet a_b_dfa').
+  Definition back_to_grammar := dfa.dfa_to_regular_grammar a_b_dfa'.
+  Eval compute in (reg_grammar.rules back_to_grammar).
+
+  (* Examples running the second DFA. *)
+  Eval compute in dfa.run a_b_dfa' [].
+  Eval compute in dfa.run a_b_dfa' [terminal.a].
+  Eval compute in dfa.run a_b_dfa' [terminal.a; terminal.a].
+  Eval compute in dfa.run a_b_dfa' [terminal.b; terminal.b].
+  Eval compute in dfa.run a_b_dfa' [terminal.a; terminal.b].
+  Eval compute in dfa.run a_b_dfa' [terminal.a; terminal.b;terminal.b].
+  Eval compute in dfa.run a_b_dfa' [terminal.b; terminal.a].
+
+  (*We can check if the automaton is a minimal automaton: *)
+  Eval compute in dfa.is_minimal a_b_dfa'.
+  Eval compute in dfa.states a_b_dfa'.
+
+  (*We can build a NFA from the DFA given above :*)
+
+  Definition nfa_from_dfa_a_b := dfa.dfa_to_nfa a_b_dfa.
+  Check dfa.dfa_to_nfa.
+  Check nfa_from_dfa_a_b.
+  Check a_b_dfa'.
+
+  Eval compute in nfa.run nfa_from_dfa_a_b [].
+  Eval compute in nfa.run nfa_from_dfa_a_b [terminal.a;terminal.a;terminal.b;terminal.a].
+  Eval compute in nfa.run nfa_from_dfa_a_b [terminal.a; terminal.a].
+  Eval compute in nfa.run nfa_from_dfa_a_b [terminal.b; terminal.b].
+  Eval compute in nfa.run nfa_from_dfa_a_b [terminal.a; terminal.b].
+  Eval compute in nfa.run nfa_from_dfa_a_b [terminal.a; terminal.b;terminal.b].
+  Eval compute in nfa.run nfa_from_dfa_a_b [terminal.b; terminal.a].
+
+  (*and we have that they run recgonize the same language *)
+  Lemma nfa_from_dfa_a_b_good : forall l, dfa.run a_b_dfa l = nfa.run nfa_from_dfa_a_b l.
+  Proof.
+  apply dfa.dfa_to_nfa_sound.
+  Qed.
+
+  (* We can also build a grammar from the automaton given above: *)
+  Definition a_b_grammar2 := dfa.dfa_to_regular_grammar a_b_dfa.
+  Eval compute in dfa.states a_b_dfa'.
+  Eval compute in dfa.alphabet a_b_dfa.
+  Eval compute in reg_grammar.rules a_b_grammar2.
+
+  Eval compute in reg_grammar.parse a_b_grammar2 [].
+  Eval compute in reg_grammar.parse a_b_grammar2 [terminal.a;terminal.b;terminal.a].
+  Eval compute in reg_grammar.parse a_b_grammar2 [terminal.b;terminal.b].
+  Eval compute in reg_grammar.parse a_b_grammar2 [terminal.a;terminal.b;terminal.b].
+
+  Inductive non_terminal1 := S| S1 | S2 | S3 |S4.
+  Inductive terminal1 := a | b |c | d.
+
+  Definition grammar_rules: list (non_terminal1 * rhs.t terminal1 non_terminal1) :=
+  [(S, Continue a S1); (S, Empty);
+     (S1, Continue b S2);
+     (S2, Continue c S3);
+     (S3, Single d);(S3, Continue a S)].
+
+  Program Instance eqdec : EqDec non_terminal1 eq :=
+      { equiv_dec x y :=
+          match x, y with
+          | S,S => in_left
+          | S1, S1 => in_left
+          | S2, S2 => in_left
+          | S3, S3 => in_left
+          | S4, S4 => in_left
+          | S, S1|S1,S| S, S2 | S2, S | S, S3 | S3, S | S1, S2 | S2, S1 | S1, S3 | S3, S1 
+          | S2, S3 | S3, S2| S4, S | S4, S1 | S4, S2 | S4, S3| S,S4 |S1, S4| S2, S4| S3,S4 => in_right
+          end
+      }.
+    Program Instance eqdec2 : EqDec terminal1 eq :=
+      { equiv_dec x y :=
+          match x, y with
+          | a,a => in_left
+          | b, b => in_left
+          | c, c => in_left
+          | d, d => in_left
+          | a, b| b,a| a, c | c, a | a, d | d, a | b, c | c, b | b, d | d, b 
+          | c, d | d, c => in_right
+          end
+      }.
+
+  Definition grammar_example := reg_grammar.build_grammar S grammar_rules
+     [a;b;c;d;a;b;c;c;c;d] [S;S1;S2;S3;S4].
+  Eval compute in reg_grammar.terminal_symbols grammar_example.
+  Definition automata_example := powerset_construction.build_dfa grammar_example.
+  Eval compute in (dfa.states automata_example).
+  Eval compute in powerset_construction.power_states grammar_example.
+
+  Eval compute in dfa.path automata_example [a;b;c;d].
+  Eval compute in dfa.run automata_example [a;b;b;c;d].
+  Eval compute in dfa.run automata_example [].
+
+  Definition rules_example_2 : set (non_terminal1 * rhs.t terminal1 non_terminal1) :=
+  [(S,Continue a S1);(S, Single a);(S,Continue b S2);(S1, Continue a S1);(S1,Continue c S3);(S2,Continue b S2);
+  (S2, Continue d S4);(S3, Single c);(S3,Continue c S);
+  (S4, Single d);(S4,Continue d S)].
+
+  (* Another example of a DFA built from a grammar: *)
+  Definition grammar_example_2 := reg_grammar.build_grammar S rules_example_2
+    [b;c;a;d] [S;S1;S2;S3;S4].
+  Definition automata_example_2 := powerset_construction.build_dfa grammar_example_2.
+  Eval compute in powerset_construction.power_states grammar_example_2.
+  Eval compute in dfa.states automata_example_2.
+
+  Eval compute in dfa.run automata_example_2 [b;d;d]. (*returns true*)
+  Eval compute in dfa.run automata_example_2 [b;d;d;c]. (*returns false*)
+  Eval compute in dfa.run automata_example_2 [a;c;c]. (*returns true*)
+  Eval compute in dfa.run automata_example_2 [a;c;c;b;d;d]. (*returns true*)
+  Eval compute in dfa.run automata_example_2 [b;d;d;a;b;c;c].    (*returns false*)
+  Eval compute in dfa.run automata_example_2 [b;b;b;b;b;b;b;d;d;a;c;c]. (*returns true*)
+  Eval compute in dfa.run automata_example_2 [b;d;d;a;c;c;b;d;d;b;d;d]. (*returns true*)
+  Eval compute in dfa.run automata_example_2 [a;a;a;a;a;a;a;c;c]. (*returns true *)
+  Eval compute in dfa.run automata_example_2 [b;a;d;a;c;c].  (*returns false*)
+
+  (* The above automaton is not minimal: *)
+  Eval compute in dfa.is_minimal automata_example_2.
+  (* Then, the list of pairs of equivalent states is an empty list. *)
+  Eval compute in dfa.check_equivalent_states automata_example_2.
+
+  Definition grammar_rules2: set (non_terminal1 * rhs.t terminal1 non_terminal1) :=
+    [(S1, Continue b S2);(S2, Continue c S3);(S3, Single d);
+     (S, Continue d S1);(S1, Continue d S1);(S1,Continue c S2);(S2, Continue b S3);
+     (S, Continue a S1);(S3, Single a);(S1, Continue a S1)].
+
+  Definition grammar := reg_grammar.build_grammar S grammar_rules2
+    [a;b;c;d] [S;S1;S2;S3].
+
+  Definition grammar_automaton := powerset_construction.build_dfa grammar.
+  Eval compute in dfa.run grammar_automaton [d;d;b;c;a].
+  Eval compute in dfa.path grammar_automaton [d;d;b;c;a].
+  Eval compute in dfa.run grammar_automaton [b].
+  Eval compute in dfa.path grammar_automaton [b].
+  Eval compute in dfa.states grammar_automaton.
+  Eval compute in dfa.is_minimal grammar_automaton.
+
+  (* Example : grammmar that have aa or bb as a subword *)
+  Definition grammar_aa_bb_rules := [(S, Continue b S); (S, Continue a S1);
+  (S1, Continue a S3);(S, Continue b S2); (S2, Continue b S3); (S3, Continue a S3);
+  (S3, Continue b S3);(S3, Empty);(S, Continue a S)].
+
+  Definition grammar_aa_bb := reg_grammar.build_grammar S grammar_aa_bb_rules
+    [a;b] [S;S1;S2;S3].
+
+  Eval compute in reg_grammar.parse grammar_aa_bb [a;a].
+  Eval compute in reg_grammar.parse grammar_aa_bb [a;b;b].
+  Eval compute in reg_grammar.parse grammar_aa_bb [a;b].
+
+  Definition automata_aa_bb := powerset_construction.build_dfa grammar_aa_bb.
+
+  Eval compute in dfa.run automata_aa_bb  [a;b;a;a;a;b].
+  Eval compute in dfa.run2 automata_aa_bb [a;b;a;a;a;b].
+  Eval compute in dfa.path automata_aa_bb [a;b;a;a;a;b].
+
+ (* ---------------------------------------------------------------------------------- *)
+ (* A hand-made NFA for the same language.                                            *)
+
+  Definition aa_bb_next (t:terminal1) (state : non_terminal1) : list non_terminal1 :=
+  match state with
+  | S => match t with
+        | a => [S;S1]
+        | b => [S;S2]
+        | c => []
+        | d => []
+        end
+  | S1 => match t with
+        | a => [S3]
+        | b => []
+        | c => []
+        | d => []
+        end
+  | S2 => match t with
+            | a => []
+            | b => [S3]
+            | c => []
+            | d => []
+            end
+  | S3 => match t with
+            | a => [S3]
+            | b => [S3]
+            | c => []
+            | d => []
+            end
+  | S4 => []
+  end.
+
+  Definition aa_bb_is_final (state: non_terminal1) : bool :=
+  match state with 
+  | S3 => true
+  | _ => false
+  end.
+
+  Definition aa_bb_nfa := {|
+    nfa.initial_state := S;
+    nfa.is_final := aa_bb_is_final;
+    nfa.next := aa_bb_next;
+    nfa.states := [S;S1;S2;S3];
+    nfa.alphabet := [a;b] |}.
+
+  Eval compute in powerset (nfa.states aa_bb_nfa).
+
+  Eval compute in nfa.path aa_bb_nfa [a;a;b;a;a;a;a;a].
+  Eval compute in nfa.run aa_bb_nfa [a;a;b;a].
+  Eval compute in nfa.run aa_bb_nfa [b;a;b;b].
+  Eval compute in nfa.path aa_bb_nfa [b;a;b;b;b;b;a].
+  Eval compute in nfa.run2 aa_bb_nfa [b;a;b;b;b;b;b;b;b].
+  Eval compute in nfa.path aa_bb_nfa [b;a;b;b;b;b;b;b;b].
+
+  (*And we can build a DFA from the NFA defined above *)
+
+  Definition aa_bb_dfa := nfa_to_dfa.build_dfa_from_nfa aa_bb_nfa.
+  (* The set of states of the DFA built from a NFA *)
+  Eval compute in (dfa.states aa_bb_dfa).
+  Eval compute in (dfa.is_minimal aa_bb_dfa).
+  Eval compute in dfa.path aa_bb_dfa [a;a].
+  Eval compute in dfa.run aa_bb_dfa [a;a;a;a;b;b].
+
+  (*NEW we can also build a grammar from the NFA defined above *)
+  Definition aa_bb_grammar := nfa.build_grammar_from_nfa aa_bb_nfa.
+  Eval compute in reg_grammar.rules aa_bb_grammar.
+  Eval compute in reg_grammar.parse aa_bb_grammar [a;a;b;a;a;a;a;a].
+
+  Definition test := [(S, Continue a S); (S, Single b)].
+
+  Definition grammar4 := reg_grammar.build_grammar S test [a;b] [S].
+
+  Eval compute in reg_grammar.rules grammar4.
+
+  Inductive naoterminal := A | B | C | D | E | F | G.
+  Inductive terminal := x|y.
+
+  Program Instance exemplo : EqDec naoterminal eq :=
+      { equiv_dec x y :=
+          match x, y with
+          | A,A => in_left
+          | B,B => in_left
+          | C,C=> in_left
+          | D,D => in_left
+          | E,E => in_left
+          | F,F => in_left
+          | G, G => in_left
+          | A,B | B,A | A,C| C, A| A,D| D,A | A,E| E,A |A,F | F,A| B,C| C,B |B ,D
+          | D,B | B,E |E,B |B,F |F,B | C,D| D,C | C,E | E,C | C,F|F,C| D,E |E,D
+          | E,F |F, E | D,F | F, D | A, G | G, A | B, G| G,B |G, C | C, G
+          | G,D| D,G |E, G |G ,E | G, F| F, G => in_right
+          end
+      }.
+
+  Program Instance exemplo2 : EqDec terminal eq :=
+    {equiv_dec x y :=
+      match x, y with
+      | x,x => in_left
+      | y,y => in_left
+      | x,y |y,x => in_right
+      end
+    }.
+
+  Definition regras := [(A, Continue a A);(A, Continue a B);(A, Continue b C); (B, Continue a D);
+  (B, Continue a E); (C, Continue a E); (C, Continue a D); (D, Continue a F);
+  (E, Continue b F); (F, Empty) ;(G, Continue c F)].
+
+  Definition gramática := reg_grammar.build_grammar A regras [a;b] [A;B;C;D;E;F;G].
+
+  Definition automato_gramatica := powerset_construction.build_dfa gramática.
+  
+  Eval compute in dfa.is_minimal automato_gramatica.
+  Eval compute in dfa.check_equivalent_states automato_gramatica.
+  Eval compute in dfa.path automato_gramatica [a].
+
+  Eval compute in dfa.run automato_gramatica [b;a;a;c].
+  Eval compute in dfa.path automato_gramatica [b;a;a;c].
+  Eval compute in dfa.run2 automato_gramatica [c].
+
+
+  (* an example of an automaton that is not minimal *)
+  Module e.
+    Inductive states := q0 |q1 | q2 |q3 | q4.
+    Inductive alphabet := a | b.
+
+    Program Instance eqstates : EqDec states eq := 
+	    {equiv_dec x y := 
+		    match x, y with 
+		    | q0,q0 => in_left 
+		    | q1,q1 => in_left 
+		    | q2,q2 => in_left 
+		    | q3,q3 => in_left 
+		    | q4,q4 => in_left 
+		    | q0,q1 => in_right 
+		    | q0,q2 => in_right 
+		    | q0,q3 => in_right 
+		    | q0,q4 => in_right 
+		    | q1,q0 => in_right 
+		    | q1,q2 => in_right 
+		    | q1,q3 => in_right 
+		    | q1,q4 => in_right 
+		    | q2,q0 => in_right 
+		    | q2,q1 => in_right 
+		    | q2,q3 => in_right 
+		    | q2,q4 => in_right 
+		    | q3,q0 => in_right 
+		    | q3,q1 => in_right 
+		    | q3,q2 => in_right 
+		    | q3,q4 => in_right 
+		    | q4,q0 => in_right 
+		    | q4,q1 => in_right 
+		    | q4,q2 => in_right 
+		    | q4,q3 => in_right 
+		    end 
+	    }.
+
+    Program Instance eqalphabet : EqDec alphabet eq :=
+      {equiv_dec x y := 
+		    match x, y with 
+        | a,a | b,b => in_left
+        | a,b | b,a => in_right
+        end
+      }.
+  End e.
+
+  Definition example_next (s: option e.states) (a: e.alphabet) :=
+    match s with
+      | None => None
+      |Some e.q0 => match a with
+               |e.a => Some e.q1
+               |e.b => None
+               end
+      |Some e.q1 => match a with
+             |e.a => Some e.q3
+             |e.b => Some e.q2
+              end
+      |Some e.q2 => match a with
+             |e.a => Some e.q4
+             |e.b => Some e.q2
+             end
+      |Some e.q3 => match a with
+             |e.a => Some e.q3
+             |e.b => Some e.q2
+              end
+      |Some e.q4 => match a with
+             |e.a => Some e.q3
+             |e.b => Some e.q2
+              end
+    end.
+
+  Definition example_is_final (s: option e.states) :=
+    match s with
+      | Some e.q4 | Some e.q3 => true
+      | None | Some _=> false
+    end.
+
+  Definition nonminimal_automaton :=
+    {| dfa.initial_state := Some e.q0;
+       dfa.is_final := example_is_final;
+       dfa.next := example_next;
+       dfa.states := [Some e.q0;Some e.q1;Some e.q2;Some e.q3;Some e.q4];
+       dfa.alphabet := [e.b;e.a] |}.
+
+  Eval compute in dfa.run nonminimal_automaton [e.a;e.b;e.a].
+  Eval compute in dfa.is_minimal nonminimal_automaton.
+  Eval compute in dfa.check_equivalent_states nonminimal_automaton.
+
+(* Examples with NFA with epsilon transitions:                        *)
+Module nfa_e_test.
+Inductive test := a | b | c.
+ Inductive test2 := q0 | q1 | q2.
+
+  Obligation Tactic := unfold complement, equiv ; program_simpl.
+  Program Instance eqdec : EqDec test eq :=
+      { equiv_dec x y :=
+          match x, y with
+          | a, a => in_left
+          | b, b => in_left
+          | c, c => in_left
+          | a,b | b,a  | a, c | c, a | b, c | c, b => in_right
+          end
+      }. 
+
+  Program Instance eqdec2 : EqDec test2 eq :=
+      { equiv_dec x y :=
+          match x, y with
+          | q0, q0 => in_left
+          | q1, q1 => in_left
+          | q2, q2 => in_left
+          | q0, q1 | q1, q0  | q0, q2 | q2, q0 | q1, q2| q2, q1 => in_right
+          end
+      }. 
+
+  Definition next_test (state: test2): set (nfa_epsilon_transitions.ep_trans test2 test) :=
+  match state with
+  | q0 => [Epsilon q1;Goes a q0]
+  | q1 => [Goes b q1; Epsilon q2]
+  | q2 => [Goes c q2]
+  end.
+
+  Eval compute in (nfa_epsilon.next_state_w_e (next_test q0)).
+
+  Definition is_f (s:test2) :=
+  match s with
+    | q2 => true
+    | _ => false
+  end.
+
+  Definition nfa_e := {|
+  nfa_epsilon.initial_state := q0;
+  nfa_epsilon.is_final := is_f;
+  nfa_epsilon.next := next_test;
+  nfa_epsilon.states := [q0;q1;q2];
+  nfa_epsilon.alphabet := [a;b;c] |}.
+
+  Eval compute in nfa_epsilon.epsilon_clos nfa_e q0. 
+  Eval compute in nfa_epsilon.epsilon_clos nfa_e q1.
+  Eval compute in nfa_epsilon.next_nfa nfa_e.
+
+  (*We can convert the above NFA with epsilon transitions to one with no *)
+  (* epsilon transitions                                                 *)
+  Definition cool_nfa_e := nfa_epsilon.nfa_e_to_nfa nfa_e.
+  Eval compute in nfa.run cool_nfa_e [a;a;a;b;c].
+
+  (* Another example:                                                    *)
+  Definition next2 (state: test2): set (nfa_epsilon_transitions.ep_trans test2 test) :=
+  match state with
+  | q0 => [Epsilon q1;Epsilon q2]
+  | q1 => [Goes b q1;Epsilon q0]
+  | q2 => [Goes c q2]
+  end.
+
+  Definition is_final2 (s:test2) :=
+    false.
+  
+  Definition nfa_e2 := {|
+  nfa_epsilon.initial_state := q0;
+  nfa_epsilon.is_final := is_final2;
+  nfa_epsilon.next := next2;
+  nfa_epsilon.states := [q0;q1;q2];
+  nfa_epsilon.alphabet := [a;b;c] |}.
+
+  Definition another_nfa_w_e := nfa_epsilon.nfa_e_to_nfa nfa_e2.
+  Eval compute in nfa_epsilon.next_nfa nfa_e2.
+
+  (*Another example *)
+  Definition next3 (state: test2): set (nfa_epsilon_transitions.ep_trans test2 test) :=
+  match state with
+  | q0 => [Epsilon q1]
+  | q1 => [Epsilon q0]
+  | q2 => []
+  end.
+  (*NFA with only two epsilon transitions between two states *)
+  Definition nfa_e3 := {|
+  nfa_epsilon.initial_state := q0;
+  nfa_epsilon.is_final := is_final2;
+  nfa_epsilon.next := next3;
+  nfa_epsilon.states := [q0;q1];
+  nfa_epsilon.alphabet := [a;b;c] |}.
+
+  Eval compute in nfa_epsilon.epsilon_clos nfa_e3 q1.
+  Eval compute in nfa_epsilon.next_nfa nfa_e3.
+End nfa_e_test.
+
